Improved this

Group.v
@@ -1,253 +1,153 @@
+Require Import Coq.Classes.SetoidClass.
+
 Definition Associative {A: Set}
+  (R: A -> A -> Prop)
   (op: A -> A -> A)
   : Prop :=
-  forall (x y z : A), op (op x y) z = op x (op y z).
-
-Definition IdentityL {A: Set}
-  (op: A -> A -> A)
-  (id: A)
-  : Prop :=
-  forall (x: A), op id x = x.
-
-Definition IdentityR {A: Set}
-  (op: A -> A -> A)
-  (id: A)
-  : Prop :=
-  forall (x: A), op x id = x.
-
-Definition Identity {A: Set}
-  (op: A -> A -> A)
-  (id: A)
-  : Prop :=
-  IdentityL op id /\ IdentityR op id.
-
-Definition InversesL {A: Set}
-  (op: A -> A -> A)
-  (id: A)
-  (inv: A -> A)
-  : Prop :=
-  forall (x: A), op (inv x) x = id.
-
-Definition InversesR {A: Set}
-  (op: A -> A -> A)
-  (id: A)
-  (inv: A -> A)
-  : Prop :=
-  forall (x: A), op x (inv x) = id.
-
-Definition Inverses {A: Set}
-  (op: A -> A -> A)
-  (id: A)
-  (inv: A -> A)
-  : Prop :=
-  InversesL op id inv /\ InversesR op id inv.
+  forall (x y z : A),
+    R (op (op x y) z) (op x (op y z)).
 
 Definition Commutative {A: Set}
+  (R: A -> A -> Prop)
   (op: A -> A -> A)
   : Prop :=
-  forall (x y : A), op x y = op y x.
+  forall (x y : A), R (op x y) (op y x).
 
-Definition IsGroup {A: Set}
-  (op: A -> A -> A)
-  (id: A)
-  (inv: A -> A)
-  : Prop :=
-  Associative op /\
-  Identity op id /\
-  Inverses op id inv.
+Class Group (A: Set) (op: A -> A -> A) : Type := {
+  #[global]
+  g_setoid :: Setoid A;
+  id : A;
+  inv : A -> A;
+  #[global]
+  op_proper :: Proper (equiv ==> equiv ==> equiv) op;
+  #[global]
+  inv_proper :: Proper (equiv ==> equiv) inv;
+  assoc : forall x y z, op (op x y) z == op x (op y z);
+  ident_l : forall x, op id x == x;
+  ident_r : forall x, op x id == x;
+  inverses_l : forall x, op (inv x) x == id;
+  inverses_r : forall x, op x (inv x) == id;
+}.
 
-Lemma apply_op_l
-  : forall (A: Set) (op: A -> A -> A) (x y : A),
-    x = y -> forall z, op z x = op z y.
+Ltac intros_refl x H :=
+  match goal with
+  | _ : Group _ _ |- _ =>
+      assert (H: x == x); [reflexivity | ..]
+  | _ => fail "must be done within group context"
+  end.
+
+Ltac op_left x H :=
+  match goal with
+  | _ : Group _ _ |- _ =>
+      let Hrefl := fresh in
+      intros_refl x Hrefl;
+      apply (op_proper x x Hrefl) in H;
+      clear Hrefl
+  | _ => fail "must be done within group context"
+  end.
+
+Ltac op_right x H :=
+  match goal with
+  | _ : Group _ _ |- _ =>
+      let Hrefl := fresh in
+      intros_refl x Hrefl;
+      apply (op_proper _ _ H) in Hrefl;
+      clear H;
+      rename Hrefl into H
+  | _ => fail "must be done within group context"
+  end.
+
+Lemma unique_id_l
+  : forall G op (Grp: Group G op) id',
+    (forall x, op id' x == x) ->
+    id' == id.
 Proof.
-  intros A op x y Heq z.
-  rewrite Heq.
-  reflexivity.
+  intros * Hid'.
+  intros_refl id H.
+  rewrite <- Hid' in H at 1.
+  rewrite ident_r in H.
+  exact H.
 Qed.
 
-Lemma apply_op_r
-  : forall (A: Set) (op: A -> A -> A) (x y : A),
-    x = y -> forall z, op x z = op y z.
+Lemma unique_id_r
+  : forall G op (Grp: Group G op) id',
+    (forall x, op x id' == x) ->
+    id' == id.
 Proof.
-  intros A op x y Heq z.
-  rewrite Heq.
-  reflexivity.
+  intros * Hid'.
+  intros_refl id H.
+  rewrite <- Hid' in H at 1.
+  rewrite ident_l in H.
+  exact H.
 Qed.
 
-Lemma unique_id
-  : forall (A: Set) (op: A -> A -> A) (id: A) (id': A),
-    Identity op id ->
-    Identity op id' ->
-    id = id'.
+Lemma unique_inv_l
+  : forall G op (Grp: Group G op) x inv',
+    op inv' x == id ->
+    inv' == inv x.
 Proof.
-  unfold Identity.
-  unfold IdentityL.
-  unfold IdentityR.
-  intros A op id id' Hid Hid'.
-  destruct Hid as [Hid _].
-  destruct Hid' as [_ Hid'].
-  specialize Hid with (x := id').
-  specialize Hid' with (x := id).
-  rewrite Hid' in Hid.
-  apply Hid.
+  intros * H.
+  op_right (inv x) H.
+  rewrite assoc in H.
+  rewrite inverses_r, ident_l, ident_r in H.
+  exact H.
 Qed.
 
-Lemma unique_inv
-  : forall (A: Set) (op: A -> A -> A) (id: A)
-      (inv: A -> A) (inv': A -> A),
-    Associative op ->
-    Identity op id ->
-    Inverses op id inv ->
-    Inverses op id inv' ->
-    forall (x: A), inv x = inv' x.
+Lemma unique_inv_r
+  : forall G op (Grp: Group G op) x inv',
+    op x inv' == id ->
+    inv' == inv x.
 Proof.
-  unfold Associative.
-  unfold Identity.
-  unfold IdentityL.
-  unfold IdentityR.
-  unfold Inverses.
-  unfold InversesL.
-  unfold InversesR.
-  intros A op id inv inv'.
-  intros Hassoc Hident Hinv Hinv' x.
-  destruct Hident as [Hident_l Hident_r].
-  destruct Hinv as [Hinv _].
-  destruct Hinv' as [_ Hinv'].
-  (* a'aa'' = a' = a'' *)
-  specialize Hinv with (x := x) as H.
-  apply apply_op_r with (op := op) (z := inv' x) in H.
-  rewrite Hident_l in H.
-  rewrite Hassoc in H.
-  rewrite Hinv' in H.
-  rewrite Hident_r in H.
-  apply H.
+  intros * H.
+  op_left (inv x) H.
+  rewrite <- assoc in H.
+  rewrite inverses_l, ident_r, ident_l in H.
+  exact H.
 Qed.
-
-Ltac unfold_isgroup HGroup
-  Hassoc Hident_l Hident_r Hinv_l Hinv_r :=
-  unfold IsGroup in HGroup;
-  unfold Associative in HGroup;
-  unfold Identity in HGroup;
-  unfold IdentityL in HGroup;
-  unfold IdentityR in HGroup;
-  unfold Inverses in HGroup;
-  unfold InversesL in HGroup;
-  unfold InversesR in HGroup;
-  destruct HGroup as
-    [Hassoc [
-    [Hident_l Hident_r]
-    [Hinv_l Hinv_r]]].
 
 Lemma cancel_l
-  : forall (A: Set) (op: A -> A -> A) (id: A) (inv: A -> A),
-    IsGroup op id inv ->
-    forall (a x y : A), op a x = op a y -> x = y.
+  : forall G op (Grp: Group G op) a x y,
+    op a x == op a y ->
+    x == y.
 Proof.
-  intros A op id inv HGroup a x y H.
-  unfold_isgroup HGroup
-    Hassoc Hident_l Hident_r Hinv_l Hinv_r.
-  apply apply_op_l with (op := op) (z := inv a) in H.
-  repeat rewrite <- Hassoc in H.
-  repeat rewrite Hinv_l in H.
-  repeat rewrite Hident_l in H.
-  apply H.
+  intros * Haxy.
+  op_left (inv a) Haxy.
+  rewrite <- 2 assoc in Haxy.
+  rewrite inverses_l in Haxy.
+  rewrite 2 ident_l in Haxy.
+  exact Haxy.
 Qed.
 
 Lemma cancel_r
-  : forall (A: Set) (op: A -> A -> A) (id: A) (inv: A -> A),
-    IsGroup op id inv ->
-    forall (a x y : A), op x a = op y a -> x = y.
-Proof.
-  intros A op id inv HGroup a x y H.
-  unfold_isgroup HGroup
-    Hassoc Hident_l Hident_r Hinv_l Hinv_r.
-  apply apply_op_r with (op := op) (z := inv a) in H.
-  repeat rewrite Hassoc in H.
-  repeat rewrite Hinv_r in H.
-  repeat rewrite Hident_r in H.
-  apply H.
+  : forall G op (Grp: Group G op) a x y,
+  op x a == op y a ->
+  x == y.
+  intros * Haxy.
+  op_right (inv a) Haxy.
+  rewrite -> 2 assoc in Haxy.
+  rewrite inverses_r in Haxy.
+  rewrite 2 ident_r in Haxy.
+  exact Haxy.
 Qed.
 
 Lemma inv_inv
-  : forall (A: Set) (op: A -> A -> A) (id: A) (inv: A -> A),
-    IsGroup op id inv ->
-    forall (x: A), inv (inv x) = x.
+  : forall G op (Grp: Group G op) x,
+    inv (inv x) == x.
 Proof.
-  intros A op id inv HGroup x.
-  unfold_isgroup HGroup
-    Hassoc Hident_l Hident_r Hinv_l Hinv_r.
-  specialize Hinv_r with (x := inv x) as H.
-  apply apply_op_l with (op := op) (z := x) in H.
-  rewrite <- Hassoc in H.
-  rewrite Hinv_r in H.
-  rewrite Hident_l in H.
-  rewrite Hident_r in H.
-  apply H.
+  intros *.
+  intros_refl id H.
+  rewrite <- (inverses_l x) in H at 2.
+  rewrite <- (inverses_r (inv x)) in H at 1.
+  apply cancel_l in H.
+  exact H.
 Qed.
 
-(*
-Require Import Nat.
+Lemma inv_op
+  : forall G op (Grp: Group G op) x y,
+    inv (op x y) == op (inv y) (inv x).
+Proof.
+  intros *.
+  intros_refl id H.
+Admitted. (* TODO *)
 
-Inductive cyclic : nat -> Set :=
-  | CZ : forall {n: nat}, cyclic (S n)
-  | CS : forall {n: nat}, cyclic n -> cyclic (S n).
-
-Check CZ : cyclic 1.
-Check CS CZ : cyclic 2.
-Check CS (CS CZ) : cyclic 3.
-Check CZ : cyclic 3.
-Fail Check CS CZ : cyclic 1.
-Check @CZ.
-Check @CS.
-
-
-Fixpoint cyclic_op
-  {n: nat}
-  (x y : cyclic n)
-  : cyclic n :=
-  match x, y with
-  | CZ, y => y
-  | CS x', y => CS (cyclic_op x' y)
-
-Definition cyclic_inv
-  (n: nat)
-  (x: nat)
-  : nat :=
-  modulo (n - (modulo x n)) n.
-
-Lemma cyclic_group
-  : forall (n: nat), IsGroup (cyclic_op n)
-
-Fixpoint repeat {A: Set}
-  (op: A -> A -> A)
-  (id: A)
-  (n: nat)
-  (x: A)
-  : A :=
-  match n with
-  | O => id
-  | S n' => op x (repeat op id n' x)
-  end.
-
-Definition Closure {A: Set}
-  (op: A -> A -> A)
-  (mem: A -> Prop)
-  : Prop :=
-  forall (x y: A), mem x -> mem y -> mem (op x y).
-
-Definition HasInverses {A: Set}
-  (inv: A -> A)
-  (mem: A -> Prop)
-  : Prop :=
-  forall (x: A), mem x -> mem (inv x).
-
-Definition IsSubgroup {A: Set}
-  (op: A -> A -> A)
-  (id: A)
-  (inv: A -> A)
-  (mem: A -> Prop)
-  : Prop :=
-  Closure op mem /\ mem id /\ HasInverses inv mem.
-
- *)
 
